Bernoulli $a=4$-el:
\Mat{
   y'=-3\tan(x)y-3\cos(x)\us
   y'=-3\tan(x)y\nh\text{homogén:}\us
   y=Ce^{-3\mint{\tan(x)}{x}}\us
   \mint{\tan(x)}{x}=-\log(|\cos(x)|)\us
   y=C|\cos(x)|^3\us
   y=C\cos^3(x)\nh \text{konstans variálás:}\us
   C'(x)\cos^3(x)-\underbrace{C(x)3\cos^2(x)\sin(x)}=\us
   = \underbrace{-3\tan(x)C(x)\cos^3(x)}-3\cos(x)\us
   C'(x)\cos^3(x)=-3\cos(x)\us
   C'(x)=-3\frac{1}{\cos^2(x)}
   C(x)=-3\tan(x)+K\us
   y(x)=(-3\tan(x)+K)\cos^3(x)\us
   u(x)=\gzjel{(-3\tan(x)+K)\cos^3(x)}^{-\frac{1}{3}}\us
}
