\Mat{
   x'=-\frac{1}{3}x+\frac{1-2t}{3}x^4 \nh \text{Bernoulli, } a=4\us
   y'=y+(2t-1)\nh y^{-\frac{1}{3}}=x\us 
   y=C(t)e^t\nh\text{:hom.mo.; C-variálás:}\us
   C'(t)=e^{-t}(2t-1)\nh \text{parciális int.:}\us
   \mint{e^{-t}(2t-1)}{t}=-e^{-t}(2t-1)-\mint{-e^{-t}2}{t}=\us
   =-e^{-t}(2t-1)-2e^{-t}=\us
   =K-e^{-t}(2t+1)\kh\text{inhom-ba vissza:}\us
   y=\gzjel{K-e^{-t}(2t+1)}e^{t}\us
   x=y^{-\frac{1}{3}}=\frac{1}{\gzjel{\gzjel{K-e^{-t}(2t+1)}e^{t} }^{\frac{1}{3}}}=\us
   =\frac{1}{\gzjel{Ke^{t}-(2t+1)}^{\frac{1}{3}}}=\us
}

