Bernoulli, $a=-2$-vel
%~ \Mat{
%~ y'=xy^{-2}+\frac{1}{x}y\kh \text{szorzás:}\kh 3y^2\us
%~ 3y^2y'=3x+\frac{3}{x}y^3\nh (z=y^3)\us
%~ z'=3x+\frac{3}{x}z\nh\text{homogén mo:}\us
%~ z=Cx^3\kh \text{variálás:}\us
%~ C'(x)x^3+C(x)3x^2=3x+3C(x)x^2\us
%~ C'(x)=3x^{-2}, \ C(x)=-3x^{-1}+K\us
%~ z=x^2(Kx-3),\ y=\gzjel{x^2(Kx-3)}^{\frac{1}{3}}
%~ }
\Mat{
y'=xy^{-2}+\frac{1}{x}y\us
u'=3\frac{1}{x}u+3x\kh\us
u'=3\frac{1}{x}u\nh \text{homogén:}\us
u=Cx^3\kh \text{változó variálás:}\us
C'(x)x^3+C(x)3x^2=3x+3C(x)x^2\us
C'(x)=3x^{-2}, \ C(x)=-3x^{-1}+K\us
u=x^2(Kx-3)\us
y=\gzjel{x^2(Kx-3)}^{\frac{1}{3}}
}


